doc/formalization/Catala.Translation.fst
@@ -3,6 +3,8 @@ module Catala.Translation
 module L = Catala.LambdaCalculus
 module D = Catala.DefaultCalculus
 
+(*** Translation definitions *)
+
 let rec translate_ty (ty: D.ty) : Tot L.ty = match ty with
   | D.TBool -> L.TBool
   | D.TUnit -> L.TUnit
@@ -16,11 +18,11 @@ let translate_lit (l: D.lit) : Tot L.lit = match l with
   | D.LConflictError -> L.LError L.ConflictError
 
 let process_exceptions_f (tau: L.ty) : Tot L.exp =
-  let a = 0 in
-  let e = 1 in
-  let e' = 2 in
-  let a' = 3 in
-  let e'' = 4 in
+  let a = -1 in
+  let e = -2 in
+  let e' = -3 in
+  let a' = -4 in
+  let e'' = -5 in
   L.EAbs a (L.TOption tau) (L.EAbs e (L.TArrow L.TUnit tau) (
     L.EApp (L.EAbs e' (L.TOption tau) (
       L.EMatchOption (L.EVar a) tau
@@ -54,11 +56,107 @@ let rec translate_exp (e: D.exp) : Tot L.exp = match e with
       (L.EFoldLeft
         (process_exceptions_f tau')
         L.ENone (L.TOption tau')
-        (L.EList (translate_exp_list exceptions)) tau')
+        (L.EList (translate_exp_list exceptions)) (L.TArrow L.TUnit tau'))
       tau'
       (L.EIf (translate_exp just) (translate_exp cons) (L.ELit (L.LError L.EmptyError)))
-      (L.EAbs 0 tau' (L.EVar 0))
+      (L.EAbs (-1) tau' (L.EVar (-1)))
 
 and translate_exp_list (l: list D.exp) : Tot (list L.exp) = match l with
   | [] -> []
-  | hd::tl -> (translate_exp hd)::(translate_exp_list tl)
+  | hd::tl -> (L.EAbs (-1) L.TUnit (translate_exp hd))::(translate_exp_list tl)
+
+let translate_env (g: D.env) : Tot L.env =
+ FunctionalExtensionality.on_dom L.var
+   (fun v -> if v < 0 then None else match g v with None -> None | Some t -> Some (translate_ty t))
+
+(*** Typing preservation *)
+
+(**** Helpers and lemmas *)
+
+let extend_translate_commute (g: D.env) (x: D.var) (tau: D.ty)
+    : Lemma (L.extend (translate_env g) x (translate_ty tau) == translate_env (D.extend g x tau))
+  =
+  FunctionalExtensionality.extensionality L.var (fun _ -> option L.ty)
+    (L.extend (translate_env g) x (translate_ty tau))
+    (translate_env (D.extend g x tau))
+
+let rec typing_preserved_by_additional_lambda_variable
+  (g: D.env) (e: L.exp) (tau: L.ty) (v: L.var{v < 0}) (tv: L.ty)
+    : Lemma
+      (requires (L.typing (translate_env g) e tau))
+      (ensures (L.typing (L.extend (translate_env g) v tv) e tau))
+  =
+  let aux = typing_preserved_by_additional_lambda_variable in
+  match e with
+  | L.EVar v' -> ()
+  | L.EApp e1 e2 tau_arg ->
+    aux g e1 (L.TArrow tau_arg tau) v tv;
+    aux g e2 tau_arg v tv
+  | L.EAbs v' tau_arg body -> begin
+    match tau with
+    | L.TArrow tau_in tau_out ->
+      if tau_in <> tau_arg then () else
+      admit()
+    | _ -> ()
+  end
+  | _ -> admit()
+
+(**** Typing preservation theorem *)
+
+#push-options "--fuel 1 --ifuel 1 --z3rlimit 30"
+let rec translation_preserves_typ (g: D.env) (e: D.exp) (tau: D.ty) : Lemma
+    (requires (D.typing g e tau))
+    (ensures (L.typing (translate_env g) (translate_exp e) (translate_ty tau)))
+    (decreases %[e; 0])
+  =
+  match e with
+  | D.EVar _ -> ()
+  | D.EApp e1 e2 tau_arg ->
+    translation_preserves_typ g e1 (D.TArrow tau_arg tau);
+    translation_preserves_typ g e2 tau_arg
+  | D.EAbs x tau_arg body -> begin
+    match tau with
+    | D.TArrow tau_in tau_out ->
+      if tau_in = tau_arg then begin
+        translation_preserves_typ (D.extend g x tau_in) body tau_out;
+        extend_translate_commute g x tau_in
+      end else ()
+    | _ -> ()
+  end
+  | D.ELit _ -> ()
+  | D.EIf e1 e2 e3 ->
+    translation_preserves_typ g e1 D.TBool;
+    translation_preserves_typ g e2 tau;
+    translation_preserves_typ g e3 tau
+  | D.EDefault exceptions just cons tau' ->
+    if tau = tau' then
+      admit()
+    else ()
+and translation_preserves_typ_exceptions
+  (g: D.env)
+  (e: D.exp)
+  (exceptions: list D.exp{exceptions << e})
+  (tau: D.ty)
+    : Lemma
+      (requires (D.typing_list g exceptions tau))
+      (ensures (L.typing_list
+        (translate_env g)
+        (translate_exp_list exceptions)
+        (L.TArrow L.TUnit (translate_ty tau))))
+      (decreases %[e; 0; exceptions])
+  =
+  match exceptions with
+  | [] -> ()
+  | hd::tl ->
+    translation_preserves_typ g hd tau;
+    translation_preserves_typ_exceptions g e tl tau;
+    let g' = translate_env g in
+    let hd' = translate_exp hd in
+    let tl' = translate_exp_list tl in
+    let tau' = translate_ty tau in
+    let thunked_tau' = L.TArrow L.TUnit tau' in
+    assert(L.typing_list g' tl' thunked_tau');
+    assert(L.typing g' hd' tau');
+    typing_preserved_by_additional_lambda_variable g hd' tau' (-1) L.TUnit;
+    assert(L.typing g' (L.EAbs (-1) L.TUnit hd') thunked_tau')
+#pop-options
